\documentclass{article}
\usepackage{amsmath}
\usepackage{kotex}
\usepackage{amssymb}  

\begin{document}

% 다항식 나눗셈 과정
\[
\begin{array}{r}
    x + 1\phantom{abcdef} \\
    x + 2{\overline{\smash{\big)}\,x^2 + 3x + 5\phantom{}}} \\
    \underline{\phantom{}x^2 + 2x\phantom{abc)}} \\
    \phantom{x^2 + }x + 5\phantom{} \\
    \underline{\phantom{}x + 2} \\
    \phantom{x^2 + 3}3\phantom{}
\end{array}
\]

% 수식 정리 과정
$$
\begin{aligned}
& x^2+3x = x(x+2) + x \\
& x+5 = 1 \cdot (x+2) + 3 \\
& \therefore x = 1 \cdot (x+2) + 3 - 5 \\
& \therefore x^2 + 3x = x(x+2) + 1 \cdot (x+2) + 3 - 5 \\
& = (x+2)\{x+1\} + 3 - 5 \\
& \therefore x^2 + 3x + 5 = (x+2)(x+1) + 3
\end{aligned}
$$

\end{document}
